rustfrontend/RustIRcfg.v
@@ -1,0 +1,487 @@
+Require Import Coqlib.
+Require Import Errors.
+Require Import Maps.
+Require Import Integers.
+Require Import Floats.
+Require Import Values.
+Require Import AST Errors.
+Require Import Memory.
+Require Import Events.
+Require Import Globalenvs.
+Require Import Smallstep.
+Require Import Ctypes Rusttypes.
+Require Import Cop RustOp.
+Require Import LanguageInterface.
+Require Import Clight Rustlight Rustlightown.
+Require Import InitDomain RustIR.
+
+Import ListNotations.
+
+(** ** Definition of selector. It is the program pointer in AST-like program.  *)
+
+Inductive select_kind : Type :=
+| Selseqleft: select_kind
+| Selseqright: select_kind
+| Selifthen: select_kind
+| Selifelse: select_kind
+| Selloop: select_kind.
+
+Definition selector := list select_kind.
+
+Fixpoint select_stmt (stmt: statement) (sel: selector) : option statement :=
+  match sel, stmt with
+  | nil, _ => Some stmt
+  | Selseqleft :: sel', Ssequence s1 s2 => select_stmt s1 sel'
+  | Selseqright :: sel', Ssequence s1 s2 => select_stmt s2 sel'
+  | Selifthen :: sel', Sifthenelse _ s1 s2 => select_stmt s1 sel'
+  | Selifelse :: sel', Sifthenelse _ s1 s2 => select_stmt s2 sel'
+  | Selloop :: sel', Sloop s => select_stmt s sel'
+  | _, _ => None
+  end.
+        
+
+(** ** Control flow graph based on selector *)
+
+Definition node := positive.
+
+(* An instruction  is either a selector or a control command (e.g., if-then-else) *)
+Inductive instruction : Type :=
+  | Inop: node -> instruction
+  | Isel: selector -> node -> instruction
+  | Icond: expr -> node -> node -> instruction
+  | Iend: instruction.
+
+Definition rustcfg := PTree.t instruction.
+
+Definition successors_instr (i: instruction) : list node :=
+  match i with
+  | Inop n => n :: nil
+  | Isel _ n => n :: nil
+  | Icond _ n1 n2 => n1 :: n2 :: nil
+  | Iend => nil
+  end.
+
+Definition get_stmt (stmt: statement) (cfg: rustcfg) (pc: node) : option statement :=
+  match cfg!pc with
+  | Some instr =>
+      match instr with
+      | Isel sel _ =>
+          select_stmt stmt sel
+      | _ => None
+      end
+  | None => None
+  end.
+
+(* Change in place the statement resided in this selector to an another
+statement. And return the modified statement *)
+Fixpoint update_stmt (root: statement) (sel: selector) (stmt: statement): option statement :=
+  match sel, root with
+  | nil, _ => Some stmt
+  | Selseqleft :: sel', Ssequence s1 s2 =>
+      match (update_stmt s1 sel' stmt) with
+      | Some s1' => Some (Ssequence s1' s2)
+      | None => None
+      end
+  | Selseqright :: sel', Ssequence s1 s2 =>      
+      match (update_stmt s2 sel' stmt) with
+      | Some s2' => Some (Ssequence s1 s2')
+      | None => None
+      end
+  | Selifthen :: sel', Sifthenelse e s1 s2 =>
+      match (update_stmt s1 sel' stmt) with
+      | Some s1' => Some (Sifthenelse e s1' s2)
+      | None => None
+      end
+  | Selifelse :: sel', Sifthenelse e s1 s2 =>
+      match (update_stmt s2 sel' stmt) with
+      | Some s2' => Some (Sifthenelse e s1 s2')
+      | None => None
+      end
+  | Selloop :: sel', Sloop s =>
+      match (update_stmt s sel' stmt) with
+      | Some s' => Some (Sloop s')
+      | None => None
+      end
+  | _, _ => None
+  end.
+
+(** ** Genenrate CFG from a statement *)
+
+(** * Translation state *)
+
+Record generator: Type := mkstate {
+  st_nextnode: node;
+  st_code: rustcfg;
+  st_wf: forall (pc: node), Plt pc st_nextnode \/ st_code!pc = None
+}.
+
+
+Inductive state_incr: generator -> generator -> Prop :=
+  state_incr_intro:
+    forall (s1 s2: generator),
+    Ple s1.(st_nextnode) s2.(st_nextnode) ->
+    (forall pc,
+        s1.(st_code)!pc = None \/ s2.(st_code)!pc = s1.(st_code)!pc) ->
+    state_incr s1 s2.
+
+Lemma state_incr_refl:
+  forall s, state_incr s s.
+Proof.
+  intros. apply state_incr_intro.
+  apply Ple_refl.
+  intros. auto.
+Qed.
+
+Lemma state_incr_trans:
+  forall s1 s2 s3, state_incr s1 s2 -> state_incr s2 s3 -> state_incr s1 s3.
+Proof.
+  intros. inv H; inv H0. apply state_incr_intro.
+  apply Ple_trans with (st_nextnode s2); assumption.
+  intros. generalize (H2 pc) (H3 pc). intuition congruence.
+Qed.
+
+(** ** The generator and error monad *)
+
+(* just copy from RTLgen *)
+
+Inductive res (A: Type) (s: generator): Type :=
+  | Err: Errors.errmsg -> res A s
+  | Res: A -> forall (s': generator), state_incr s s' -> res A s.
+
+Arguments Res [A s].
+Arguments Err [A s].
+
+Definition mon (A: Type) : Type := forall (s: generator), res A s.
+
+Definition ret {A: Type} (x: A) : mon A :=
+  fun (s: generator) => Res x s (state_incr_refl s).
+
+
+Definition error {A: Type} (msg: Errors.errmsg) : mon A := fun (s: generator) => Err msg.
+
+Definition bind {A B: Type} (f: mon A) (g: A -> mon B) : mon B :=
+  fun (s: generator) =>
+    match f s with
+    | Err msg => Err msg
+    | Res a s' i =>
+        match g a s' with
+        | Err msg => Err msg
+        | Res b s'' i' => Res b s'' (state_incr_trans s s' s'' i i')
+        end
+    end.
+
+Definition bind2 {A B C: Type} (f: mon (A * B)) (g: A -> B -> mon C) : mon C :=
+  bind f (fun xy => g (fst xy) (snd xy)).
+
+Declare Scope cfg_monad_scope.
+Notation "'do' X <- A ; B" := (bind A (fun X => B))
+   (at level 200, X ident, A at level 100, B at level 200): cfg_monad_scope.
+Notation "'do' ( X , Y ) <- A ; B" := (bind2 A (fun X Y => B))
+   (at level 200, X ident, Y ident, A at level 100, B at level 200): cfg_monad_scope.
+
+Definition handle_error {A: Type} (f g: mon A) : mon A :=
+  fun (s: generator) =>
+    match f s with
+    | Res a s' i => Res a s' i
+    | Err _ => g s
+    end.
+
+
+
+(** ** Operations on generator *)
+
+(** The initial generator (empty CFG). *)
+
+Remark init_state_wf:
+  forall pc, Plt pc 1%positive \/ (PTree.empty instruction)!pc = None.
+Proof. intros; right; apply PTree.gempty. Qed.
+
+Definition init_state : generator :=
+  mkstate 1%positive (PTree.empty instruction) init_state_wf.
+
+
+Remark add_instr_wf:
+  forall s i pc,
+  let n := s.(st_nextnode) in
+  Plt pc (Pos.succ n) \/ (PTree.set n i s.(st_code))!pc = None.
+Proof.
+  intros. case (peq pc n); intro.
+  subst pc; left; apply Plt_succ.
+  rewrite PTree.gso; auto.
+  elim (st_wf s pc); intro.
+  left. apply Plt_trans_succ. exact H.
+  right; assumption.
+Qed.
+
+Remark add_instr_incr:
+  forall s i,
+  let n := s.(st_nextnode) in
+  state_incr s (mkstate (Pos.succ n)
+                  (PTree.set n i s.(st_code))
+                  (add_instr_wf s i)).
+Proof.
+  constructor; simpl.
+  apply Ple_succ.
+  intros. destruct (st_wf s pc). right. apply PTree.gso. apply Plt_ne; auto. auto.
+Qed.
+
+Definition add_instr (i: instruction) : mon node :=
+  fun s =>
+    let n := s.(st_nextnode) in
+    Res n
+       (mkstate (Pos.succ n) (PTree.set n i s.(st_code))
+                (add_instr_wf s i))
+       (add_instr_incr s i).
+
+(** [add_instr] can be decomposed in two steps: reserving a fresh
+  CFG node, and filling it later with an instruction.  This is needed
+  to compile loops. *)
+
+Remark reserve_instr_wf:
+  forall s pc,
+  Plt pc (Pos.succ s.(st_nextnode)) \/ s.(st_code)!pc = None.
+Proof.
+  intros. elim (st_wf s pc); intro.
+  left; apply Plt_trans_succ; auto.
+  right; auto.
+Qed.
+
+Remark reserve_instr_incr:
+  forall s,
+  let n := s.(st_nextnode) in
+  state_incr s (mkstate (Pos.succ n)
+                  s.(st_code)
+                      (reserve_instr_wf s)).
+Proof.
+  intros; constructor; simpl.
+  apply Ple_succ.
+  auto.
+Qed.
+
+Definition reserve_instr: mon node :=
+  fun (s: generator) =>
+  let n := s.(st_nextnode) in
+  Res n
+     (mkstate (Pos.succ n) s.(st_code) (reserve_instr_wf s))
+     (reserve_instr_incr s).
+
+Remark update_instr_wf:
+  forall s n i,
+  Plt n s.(st_nextnode) ->
+  forall pc,
+  Plt pc s.(st_nextnode) \/ (PTree.set n i s.(st_code))!pc = None.
+Proof.
+  intros.
+  case (peq pc n); intro.
+  subst pc; left; assumption.
+  rewrite PTree.gso; auto. exact (st_wf s pc).
+Qed.
+
+Remark update_instr_incr:
+  forall s n i (LT: Plt n s.(st_nextnode)),
+  s.(st_code)!n = None ->
+  state_incr s
+             (mkstate s.(st_nextnode) (PTree.set n i s.(st_code))
+                     (update_instr_wf s n i LT)).
+Proof.
+  intros.
+  constructor; simpl; intros.
+  apply Ple_refl.
+  rewrite PTree.gsspec. destruct (peq pc n). left; congruence. right; auto.
+Qed.
+
+Definition check_empty_node:
+  forall (s: generator) (n: node), { s.(st_code)!n = None } + { True }.
+Proof.
+  intros. case (s.(st_code)!n); intros. right; auto. left; auto.
+Defined.
+
+Definition update_instr (n: node) (i: instruction) : mon unit :=
+  fun s =>
+    match plt n s.(st_nextnode), check_empty_node s n with
+    | left LT, left EMPTY =>
+        Res tt
+           (mkstate s.(st_nextnode) (PTree.set n i s.(st_code))
+                    (update_instr_wf s n i LT))
+           (update_instr_incr s n i LT EMPTY)
+    | _, _ =>
+        Err (Errors.msg "RTLgen.update_instr")
+    end. 
+
+
+Local Open Scope cfg_monad_scope.
+
+(** Translation of statement *)
+
+Section COMPOSITE_ENV.
+
+Variable (ce: composite_env).
+
+Import ListNotations.
+
+Fixpoint transl_stmt (end_node: node) (stmt: statement) (sel: selector) (succ: node) (cont: option node) (brk: option node) {struct stmt} : mon node :=
+  let transl_stmt := transl_stmt end_node in
+  match stmt with
+  | Sskip =>
+      add_instr (Isel sel succ)
+  | Sassign p e =>
+      add_instr (Isel sel succ)
+  | Sassign_variant p enum_id fid e =>
+      add_instr (Isel sel succ)
+  | Sbox p e =>
+      add_instr (Isel sel succ)
+  | Ssequence stmt1 stmt2 =>
+      do succ2 <- transl_stmt stmt2 (sel ++ [Selseqright]) succ cont brk;
+      do succ1 <- transl_stmt stmt1 (sel ++ [Selseqleft]) succ2 cont brk;
+      ret succ1
+  | Sifthenelse e stmt1 stmt2 =>
+      do n1 <- transl_stmt stmt1 (sel ++ [Selifthen]) succ cont brk;
+      do n2 <- transl_stmt stmt2 (sel ++ [Selifelse]) succ cont brk;
+      do n3 <- add_instr (Icond e n1 n2);
+      ret n3
+  | Sloop stmt =>
+      do loop_jump_node <- reserve_instr;
+      (* The succ in function body is loop_start *)
+      do body_start <- transl_stmt stmt (sel ++ [Selloop]) loop_jump_node (Some loop_jump_node) (Some succ);
+      do _ <- update_instr loop_jump_node (Inop body_start);
+      (* return loop_jump_node and return body_start are equivalent *)
+      ret loop_jump_node
+  | Sbreak =>
+      match brk with
+      | None =>
+          error (Errors.msg "No loop outside the break: transl_stmt")
+      | Some brk =>
+          add_instr (Inop brk)
+      end
+  | Scontinue =>
+      match cont with
+      | None =>
+          error (Errors.msg "No loop outside the continue")
+      | Some cont =>
+          add_instr (Inop cont)
+      end
+  | Sstoragelive id =>
+      add_instr (Isel sel succ)
+  | Sstoragedead id =>
+      add_instr (Isel sel succ)
+  | Sdrop p =>
+      add_instr (Isel sel succ)
+  | Scall p a al =>
+      add_instr (Isel sel succ)
+  | Sreturn e =>
+      add_instr (Isel sel end_node)
+    end.
+
+Definition generate_cfg' (stmt: statement): mon node :=
+  (* return node *)
+  do return_node <- add_instr Iend;
+  transl_stmt return_node stmt nil return_node None None.
+
+Definition generate_cfg (stmt: statement): Errors.res (node * rustcfg) :=  
+  match generate_cfg' stmt init_state with
+  | Res start st _ =>
+      Errors.OK (start, st.(st_code))
+  | Err msg =>
+      Errors.Error msg
+  end.
+  
+
+End COMPOSITE_ENV.
+
+
+(** * Relations between the generated CFG and the source statement *)
+
+(* Translation relation of the generate_cfg: [tr_stmt body cfg stmt pc
+  out cont break endn] holds if the graph [cfg], starting at node
+  [pc], contains instructions that perform the RustIR statement
+  [stmt]. These instructions branch to node [out] if the statement
+  terminates normally, branch to node [cont] if the statement reaches
+  Scontinue, branch to break if the statement reaches Sbreak and
+  branch to [endn] if the statement returns *)
+Inductive tr_stmt (body: statement) (cfg: rustcfg) : statement -> node -> node -> option node -> option node -> node -> Prop :=
+| tr_Sskip: forall pc cont brk endn,
+    tr_stmt body cfg Sskip pc pc cont brk endn
+| tr_Sassign: forall pc next sel p e cont brk endn
+    (SEL: cfg ! pc = Some (Isel sel next))
+    (STMT: select_stmt body sel = Some (Sassign p e)),
+    tr_stmt body cfg (Sassign p e) pc next cont brk endn
+| tr_Sassign_variant: forall pc next sel p e enum_id fid cont brk endn
+    (SEL: cfg ! pc = Some (Isel sel next))
+    (STMT: select_stmt body sel = Some (Sassign_variant p enum_id fid e)),
+    tr_stmt body cfg (Sassign_variant p enum_id fid e) pc next cont brk endn
+| tr_Sbox: forall pc next sel p e cont brk endn
+    (SEL: cfg ! pc = Some (Isel sel next))
+    (STMT: select_stmt body sel = Some (Sbox p e)),
+    tr_stmt body cfg (Sbox p e) pc next cont brk endn
+| tr_Sstoragelive: forall pc next sel id cont brk endn
+    (SEL: cfg ! pc = Some (Isel sel next))
+    (STMT: select_stmt body sel = Some (Sstoragelive id)),
+    tr_stmt body cfg (Sstoragelive id) pc next cont brk endn
+| tr_Sstoragedead: forall pc next sel id cont brk endn
+    (SEL: cfg ! pc = Some (Isel sel next))
+    (STMT: select_stmt body sel = Some (Sstoragedead id)),
+    tr_stmt body cfg (Sstoragedead id) pc next cont brk endn
+| tr_Sdrop: forall pc next sel p cont brk endn
+    (SEL: cfg ! pc = Some (Isel sel next))
+    (STMT: select_stmt body sel = Some (Sdrop p)),
+    tr_stmt body cfg (Sdrop p) pc next cont brk endn
+| tr_Scall: forall pc next sel p e args cont brk endn
+    (SEL: cfg ! pc = Some (Isel sel next))
+    (STMT: select_stmt body sel = Some (Scall p e args)),
+    tr_stmt body cfg (Scall p e args) pc next cont brk endn
+| tr_Ssequence: forall s1 s2 n1 n2 n3 cont brk endn
+    (STMT1: tr_stmt body cfg s1 n1 n2 cont brk endn)
+    (STMT2: tr_stmt body cfg s2 n2 n3 cont brk endn),
+    tr_stmt body cfg (Ssequence s1 s2) n1 n3 cont brk endn
+| tr_Sifthenelse: forall s1 s2 e pc n1 n2 endif cont brk endn
+    (STMT1: tr_stmt body cfg s1 n1 endif cont brk endn)
+    (STMT2: tr_stmt body cfg s2 n2 endif cont brk endn)
+    (SEL: cfg ! pc = Some (Icond e n1 n2)),
+    tr_stmt body cfg (Sifthenelse e s1 s2) pc endif cont brk endn
+| tr_Sloop: forall s next loop_start loop_jump_node cont brk endn
+    (STMT: tr_stmt body cfg s loop_start loop_jump_node (Some loop_jump_node) (Some next) endn)
+    (SEL: cfg ! loop_jump_node = Some (Inop loop_start)),
+    (* next is not specific because loop is impossible to terminate
+    normally *)
+    tr_stmt body cfg (Sloop s) loop_jump_node next brk cont endn
+| tr_Sbreak: forall pc brk cont endn
+    (SEL: cfg ! pc = Some (Inop brk)),
+    tr_stmt body cfg Sbreak pc brk cont (Some brk) endn
+| tr_Scontinue: forall pc brk cont endn
+    (SEL: cfg ! pc = Some (Inop cont)),
+    tr_stmt body cfg Scontinue pc cont (Some cont) brk endn
+| tr_Sreturn: forall pc sel endn e cont brk
+    (SEL: cfg ! pc = Some (Isel sel endn))
+    (STMT: select_stmt body sel = Some (Sreturn e)),
+    tr_stmt body cfg (Sreturn e) pc endn cont brk endn
+.
+
+Inductive tr_fun (f: function) (nret: node) : rustcfg -> Prop :=
+| tr_fun_intro: forall entry cfg
+    (CFG: generate_cfg f.(fn_body) = OK (entry, cfg))
+    (STMT: tr_stmt f.(fn_body) cfg f.(fn_body) entry nret None None nret),
+    tr_fun f nret cfg.
+
+
+(* tr_stmt matches transl_stmt *)
+Lemma transl_stmt_charact: forall body sel stmt nret succ cont brk s s' n R,
+    select_stmt body sel = Some stmt ->
+    transl_stmt nret stmt sel succ cont brk s = Res n s' R ->
+    tr_stmt body s'.(st_code) stmt n succ cont brk nret.
+Admitted.
+
+
+Lemma generate_cfg_charact: forall f entry cfg,
+    generate_cfg f.(fn_body) = OK (entry, cfg) ->
+    exists nret, tr_fun f nret cfg.
+Proof.
+  intros f entry cfg GEN.
+  generalize GEN. intros GEN'.
+  unfold generate_cfg in GEN.
+  destruct (generate_cfg' (fn_body f) init_state) eqn: GCFG; try congruence.
+  inv GEN. unfold generate_cfg' in GCFG.
+  (** TODO: copy some monadInv from RTLgenspec.v *)
+Admitted.
+
+                              
+                             
